language_formal/spark2014_semantics/spark2014_core_subset(non-nested)/symboltable.v
@@ -1,0 +1,126 @@
+Require Export language.
+Require Export environment.
+
+Definition level := nat.
+
+(* each procedure declaration is associated with a scope level, 
+   which can be used to determine what variables are visible to 
+   the procedure when it's called;
+*)
+Record symboltable := mkSymbolTable{
+  vars:   list (idnum * (mode * type));
+  procs: list (procnum * (level * procedure_declaration));
+  types:  list (typenum * type_declaration)
+}.
+
+Module Entry_Type <: ENTRY.
+
+  Definition T := prod mode type.
+
+End Entry_Type.
+
+Module Entry_Procedure_Decl <: ENTRY.
+
+  Definition T := prod level procedure_declaration.
+
+End Entry_Procedure_Decl.
+
+Module Entry_Type_Decl <: ENTRY.
+
+  Definition T := type_declaration.
+
+End Entry_Type_Decl.
+
+Module SymTable_Vars  := STORE(Entry_Type).
+Module SymTable_Procs := STORE(Entry_Procedure_Decl).
+Module SymTable_Types := STORE(Entry_Type_Decl).
+
+Function reside_symtable_vars  (x: idnum)   (st: symboltable) := SymTable_Vars.resides x st.(vars).
+Function reside_symtable_procs (x: procnum) (st: symboltable) := SymTable_Procs.resides x st.(procs).
+Function reside_symtable_types (x: typenum) (st: symboltable) := SymTable_Types.resides x st.(types).
+
+Function fetch_var  (x: idnum)   (st: symboltable) := SymTable_Vars.fetches x st.(vars).
+Function fetch_proc (x: procnum) (st: symboltable) := SymTable_Procs.fetches x st.(procs).
+Function fetch_type (x: typenum) (st: symboltable) := SymTable_Types.fetches x st.(types).  
+
+Function update_store {V} (s: list (idnum * V)) (i: idnum) (v: V): list (idnum * V) :=
+  match s with 
+  | (i1, v1) :: s1 =>
+      if beq_nat i1 i then
+        (i1, v) :: s1
+      else
+        (i1, v1) :: (update_store s1 i v)
+  | nil => (i, v) :: nil
+  end.
+
+Arguments update_store {V} _ _ _.
+
+Function update_vars (st: symboltable) (x: idnum) (mt: mode * type): symboltable :=
+  mkSymbolTable (update_store st.(vars) x mt) st.(procs) st.(types).
+
+Function update_procs (st: symboltable) (pid: procnum) (p: level * procedure_declaration): symboltable :=
+  mkSymbolTable st.(vars) (update_store st.(procs) pid p) st.(types).
+
+Function update_types (st: symboltable) (tid: typenum) (td: type_declaration): symboltable :=
+  mkSymbolTable st.(vars) st.(procs) (update_store st.(types) tid td).
+
+
+
+(* **********************************
+   build symbol table from SPARK AST 
+   ********************************** *)
+
+
+(*
+Inductive symboltable_decl: symboltable -> context -> declaration -> symboltable -> Prop :=
+
+.
+
+Inductive symboltable_subprogram: symboltable -> context -> subprogram -> symboltable
+  | ST_Procedure: 
+       
+      symboltable_subprogram st1 (Global_Procedure ast_num pd) st2.
+
+*)
+
+
+
+
+
+
+
+
+
+
+
+
+
+
+
+
+
+
+
+
+
+
+
+
+
+
+
+
+
+
+
+
+
+
+
+
+
+
+
+
+
+
